src/FiatToFacade/Loop.v
@@ -1,6 +1,6 @@
 Require Import StringMap.
 Require Import Memory.
-Require Import Facade.FacadeADTs.
+Require Import Facade.examples.FiatADTs.
 Require Import FiatToFacade.FacadeNotations.
 Require Import FiatToFacade.Prog FiatToFacade.StringMapNotations.
 
@@ -35,3 +35,19 @@ Definition ADTLoopBodyOk
   forall acc (head: W) (seq: list W),
     @ADTLoopBodyProgCondition env acc_type loop compiled_loop knowledge scas adts vseq
                               vret thead tis_empty acc wrapper head seq.
+
+Definition PairLoopBodyProgCondition
+           env {acc_type} loop compiled_loop knowledge scas adts
+           (vseq vsca vadt thead tis_empty: StringMap.key) (acc: acc_type) wsca wadt (head: W) (seq: list W) :=
+  @ProgOk _ env compiled_loop knowledge
+          ([thead >sca> head]::[tis_empty >sca> 0]::[vsca >sca> wsca acc]::scas)
+          ([vsca >sca> wsca (loop acc head)]::scas)
+          ([vadt >adt> wadt acc]::[vseq >adt> List seq]::adts)
+          ([vadt >adt> wadt (loop acc head)]::[vseq >adt> List seq]::adts).
+
+Definition PairLoopBodyOk
+           env {acc_type} loop compiled_loop knowledge scas adts
+           (vseq vsca vadt thead tis_empty: StringMap.key) wsca wadt :=
+  forall acc (head: W) (seq: list W),
+    @PairLoopBodyProgCondition env acc_type loop compiled_loop knowledge scas adts
+                               vseq vsca vadt thead tis_empty acc wsca wadt head seq.
