src/FiatToFacade/Compiler.v
@@ -1,0 +1,53 @@
+Require Export
+        FiatToFacade.Compiler.Prerequisites
+        FiatToFacade.Compiler.Utilities
+        FiatToFacade.Compiler.Basics
+        FiatToFacade.Compiler.Constants
+        FiatToFacade.Compiler.NoOp
+        FiatToFacade.Compiler.Copy
+        FiatToFacade.Compiler.Binops
+        FiatToFacade.Compiler.Pairs
+        FiatToFacade.Compiler.Cleanup
+        FiatToFacade.Compiler.Conditionals
+        FiatToFacade.Compiler.ADTs.Folds
+        FiatToFacade.Compiler.ADTs.Lists
+        FiatToFacade.Compiler.ADTs.ListsInversion
+        FiatToFacade.Compiler.ADTs.FiniteSets.
+
+Require Export Common.
+Require Export Facade.Facade.
+Require Export Facade.DFacade.
+Require Export Facade.examples.FiatADTs.
+Require Export Cito.StringMap.
+Require Export Cito.GLabelMap.
+
+Definition AddPair {av} pair m :=
+  @GLabelMap.add (FuncSpec av) (fst pair) (snd pair) m.
+
+Definition MakePair {av} (k: GLabel.glabel) (v: AxiomaticSpec av) :=
+  (k, Axiomatic v).
+
+Notation "[[[ p1 ; .. ; pn ]]]" :=
+  (AddPair p1 .. (AddPair pn (GLabelMap.empty _)) ..).
+
+Notation "k ↦ v" :=
+  (MakePair k v) (at level 55, no associativity).
+
+Definition empty_env {av} := GLabelMap.empty (FuncSpec av).
+                                                      
+Definition basic_env := [[[ ("List", "empty") ↦ List_empty;
+                            ("List", "Pop") ↦ List_pop;
+                            ("List", "New") ↦ List_new;
+                            ("List", "Push") ↦ List_push;
+                            ("List", "Copy") ↦ List_copy;
+                            ("List", "Delete") ↦ List_delete ]]].
+
+Unset Implicit Arguments.
+
+Definition start_adt state vret {ret_type v} wrapper wrapper_inj adts :=
+  (@start_compiling_adt_with_precondition _ basic_env state ∅ adts vret ret_type v wrapper wrapper_inj).
+
+Definition start_sca state vret adts :=
+  (@start_compiling_sca_with_precondition _ basic_env state ∅ adts vret).
+
+Notation refine' := refine.
